Added some preliminary examples of Lowenheim's formula running

B-unification/lowenheim.v
@@ -25,8 +25,7 @@ Definition tau (b : bool) : term :=
 
 (* Creates a single replacement (var -> term) for lowenheim's formula *)
 Definition lowenheim_replace (t : term) (v : var) (b : bool) : replacement :=
-  if (term_contains_var t v) then (v, (t + T1) * VAR v + t * (tau b))
-  else (v, VAR v).
+  (v, (t + T1) * VAR v + t * (tau b)).
 
 (* Creates a substitution (list replacement) for lowenheim's formula. Any variables entered into vars will be 
    set to 1 *)
@@ -35,3 +34,61 @@ Fixpoint lowenheim_subst (t : term) (term_vars : var_set) (vars : var_set) : sub
     | nil => nil (* Can't create a substitution for a term with no variables! *)
     | v :: v' => (lowenheim_replace t v (var_set_includes_var v vars)) :: (lowenheim_subst t v' vars)
   end.
+
+(* Lowenheim's formula *)
+Definition lowenheim (t : term) (vars : var_set) : subst :=
+  lowenheim_subst t (term_unique_vars t) vars.
+
+Example lowenheim_ex1 :
+  mgu (VAR 0 * VAR 1) (lowenheim (VAR 0 * VAR 1) ([0;1])).
+Proof.
+unfold mgu. intros. unfold lowenheim. simpl in *.
+unfold more_general_subst. intros. unfold lowenheim_replace. simpl.
+inversion H.
+Qed.
+
+Example lowenheim_ex2 :
+  mgu (VAR 0 * VAR 1) (lowenheim (VAR 0 * VAR 1) ([0])).
+Proof.
+unfold mgu. intros. unfold lowenheim. simpl in *.
+unfold more_general_subst. intros. unfold lowenheim_replace. simpl.
+inversion H.
+Qed.
+
+Example lowenheim_ex3 :
+  mgu (VAR 0 * VAR 1) (lowenheim (VAR 0 * VAR 1) ([1])).
+Proof.
+unfold mgu. intros. unfold lowenheim. simpl in *.
+unfold more_general_subst. intros. unfold lowenheim_replace. simpl.
+inversion H.
+Qed.
+
+Example lowenheim_ex4 :
+  mgu (VAR 0 * VAR 1) (lowenheim (VAR 0 * VAR 1) ([])).
+Proof.
+unfold mgu. intros. unfold lowenheim. simpl in *.
+unfold more_general_subst. intros. unfold lowenheim_replace. simpl.
+inversion H.
+Qed.
+
+(* Proof of lowenheim's formula *)
+Theorem lowenheim_generates_mgus :
+  forall t vars, (solve t vars = T0) -> (mgu t (lowenheim t vars)).
+Proof.
+intros. induction t, vars. 
+{ simpl in *. unfold mgu. intros. unfold more_general_subst. intros. simpl.
+  reflexivity. }
+{ simpl in *. unfold mgu. intros. unfold more_general_subst. intros. simpl.
+  reflexivity. }
+{ simpl in *. unfold mgu. intros. unfold more_general_subst. intros. simpl.
+  reflexivity. }
+{ simpl in *. unfold mgu. intros. unfold more_general_subst. intros. simpl.
+  reflexivity. }
+{ simpl in *. unfold mgu. intros. unfold more_general_subst. intros. simpl.
+  unfold lowenheim in H0. simpl in *.
+Admitted.
+
+
+
+
+
