B-unification/terms.v
@@ -471,4 +471,3 @@ unfold unifier in *. simpl in *. induction s_prime.
 { simpl in *. inversion H. }
 { simpl. inversion H. }
 Qed.
-
